small renamings

theories/NP/TM/TMGenNP_fixed_mTM.v
@@ -1,24 +1,31 @@
 From Undecidability.TM Require Import TM_facts.
 From Undecidability.L.TM Require Import TMEncoding.
-From Complexity.Complexity Require Import NP.
+From Complexity.Complexity Require Import NP Subtypes.
 From Undecidability.L Require Import Tactics.LTactics.
 
 (** For each Machine M (with n+1 tapes), we define this problem:
 Given n tapes and a sizeBound and a step bound, does there exist a (small enough) first tape such that the machine halts on the resulting n+1 tapes in fewer steps than the step bound? *)
 
 (** We contain this on haltsOrDiverges as our MutiTape2SingleTape-translation probably only knows upper bounds of the step count.  *)
-Definition HaltsOrDiverges_fixed_mTM (sig : finType) `{encodable sig} n (M : TM sig (S n)) : Vector.t (tape sig) n * nat * nat -> Prop :=
-  fun '(ts, maxSize, steps) =>
-    forall t__cert' k res', loopM (initc M (t__cert':::ts)) k = Some res'
-                     -> exists t__cert res, sizeOfTape t__cert <= maxSize
-                                    /\ loopM (initc M (t__cert:::ts)) steps = Some res.
+Section mTM.
+  Context {sig : finType} {n} (M : TM sig (S n)).
 
-Definition TMGenNP_fixed_mTM (sig : finType) `{encodable sig} n (M : TM sig (S n))
-  := (fun '(ts, maxSize, steps) =>
-        exists t1, sizeOfTape t1 <= maxSize /\ exists f, loopM (initc M (t1:::ts)) steps = Some f).
+  Definition HaltsOrDiverges_mTM_fixed : Vector.t (tape sig) n * nat * nat -> Prop :=
+    fun '(ts, maxSize, steps) =>
+      forall t__cert' k res', loopM (initc M (t__cert':::ts)) k = Some res'
+                      -> exists t__cert res, sizeOfTape t__cert <= maxSize
+                                      /\ loopM (initc M (t__cert:::ts)) steps = Some res.
 
-Arguments TMGenNP_fixed_mTM : clear implicits.
-Arguments TMGenNP_fixed_mTM {_ _ _}.
+  Definition mTMGenNP_fixed' := (fun '(ts, maxSize, steps) =>
+          exists t1, sizeOfTape t1 <= maxSize /\ exists f, loopM (initc M (t1:::ts)) steps = Some f).
+
+  Definition mTMGenNP_fixed : {x | HaltsOrDiverges_mTM_fixed x} -> Prop :=
+    restrictBy HaltsOrDiverges_mTM_fixed mTMGenNP_fixed'.
+
+End mTM.
+
+Arguments mTMGenNP_fixed {_ _} _.
+
 
 Definition initTape_singleTapeTM (sig : Type) (s : list sig) :=
   match s with
@@ -26,10 +33,8 @@ Definition initTape_singleTapeTM (sig : Type) (s : list sig) :=
     | x::s => @leftof sig x s
   end. 
 
-Definition TMGenNP_fixed_singleTapeTM (sig : finType) `{encodable sig} (M : TM sig 1)
+Definition TMGenNP_fixed {sig : finType} (M : TM sig 1)
   := (fun '(ts, maxSize, steps) =>
         exists (cert : list sig), length cert <= maxSize
-                             /\ exists res, execTM M [|initTape_singleTapeTM (ts++cert)|] steps = Some res).
+                            /\ exists res, execTM M [|initTape_singleTapeTM (ts++cert)|] steps = Some res).
 
-Arguments TMGenNP_fixed_singleTapeTM : clear implicits.
-Arguments TMGenNP_fixed_singleTapeTM {_ _}.
